Add the remaining theorems for `Option`
This commit adds statements and proofs of the remaining theorems to
accompany the functionality of the `std::option::Option<T>` type. It
also introduces a document that aims to collate useful tips for stating
theorems and proving.

stdlib/lampe/Stdlib/Option.lean
@@ -33,29 +33,22 @@ open «std-1.0.0-beta.11».Extracted
 set_option maxRecDepth 1000
 
 def from_option {p t}: Option (t.denote p) -> («std::option::Option».tp h![t] |>.denote p)
-| none => (false, Lampe.Tp.zero p t, ())
+| none => (false, Tp.zero p t, ())
 | some val => (true, val, ())
 
-def to_option {p t}: («std::option::Option».tp h![t] |>.denote p) -> Option (t.denote p)
-| (false, _, _) => none
-| (true, val, _) => some val
-
-lemma from_option_to_option_id : to_option (from_option v) = v := by
-  cases v <;> rfl
-
-lemma none_spec {p T} : Lampe.STHoare p env ⟦⟧ («std::option::Option::none».call h![T] h![]) 
+theorem none_spec {p T} : STHoare p env ⟦⟧ («std::option::Option::none».call h![T] h![]) 
     (fun v => v = from_option none) := by
   enter_decl
   steps
   assumption
 
-lemma some_spec {p T v} : Lampe.STHoare p env ⟦⟧ («std::option::Option::some».call h![T] h![v])
+theorem some_spec {p T v} : STHoare p env ⟦⟧ («std::option::Option::some».call h![T] h![v])
     (fun r => r = from_option (some v)) := by
   enter_decl
   steps
   assumption
 
-lemma is_none_spec {p T v} : Lampe.STHoare p env ⟦⟧ 
+theorem is_none_spec {p T v} : STHoare p env ⟦⟧ 
     («std::option::Option::is_none».call h![T] h![from_option v]) 
     (fun r => r = v.isNone) := by
   enter_decl
@@ -64,7 +57,7 @@ lemma is_none_spec {p T v} : Lampe.STHoare p env ⟦⟧
   cases v <;> rfl
   exact ()
 
-lemma is_some_spec {p T v} : Lampe.STHoare p env ⟦⟧ 
+theorem is_some_spec {p T v} : STHoare p env ⟦⟧ 
     («std::option::Option::is_some».call h![T] h![from_option v]) 
     (fun r => r = v.isSome) := by
   enter_decl
@@ -72,7 +65,7 @@ lemma is_some_spec {p T v} : Lampe.STHoare p env ⟦⟧
   subst_vars
   cases v <;> rfl
 
-lemma unwrap_spec {p T v} : Lampe.STHoare p env ⟦⟧ 
+theorem unwrap_spec {p T v} : STHoare p env ⟦⟧ 
     («std::option::Option::unwrap».call h![T] h![from_option v]) 
     (fun r => ∃h, r = v.get h) := by
   enter_decl
@@ -85,36 +78,73 @@ lemma unwrap_spec {p T v} : Lampe.STHoare p env ⟦⟧
     simp
     rfl
 
-lemma map_none_spec {p T U E f} : Lampe.STHoare p env ⟦⟧ 
-  («std::option::Option::map».call h![T, U, E] h![from_option none, f]) 
-  (fun r => r = from_option (none: Option (U.denote p))) := by
+theorem map_none_spec {p T U E f} : STHoare p env ⟦⟧ 
+    («std::option::Option::map».call h![T, U, E] h![from_option none, f]) 
+    (fun r => r = from_option (none: Option (U.denote p))) := by
   enter_decl
   steps
-  apply Lampe.STHoare.iteFalse_intro
+  apply STHoare.iteFalse_intro
   steps [none_spec]
   assumption
 
-lemma map_some_spec {p T U E f fb v P Q}
-    (h_lam : Lampe.STHoare p env P (fb h![v]) Q):
-    Lampe.STHoare p env
-      (P ⋆ [λf ↦ fb])
-      («std::option::Option::map».call h![T, U, E] h![from_option (some v), f])
-      (fun v => (∃∃vin, v = (from_option (some vin)) ⋆ Q vin) ⋆ [λf ↦ fb]) := by
+theorem map_some_spec {p T U E f fb v P Q}
+    (h_lam : STHoare p env P (fb h![v]) Q)
+  : STHoare p env
+    (P ⋆ [λf ↦ fb])
+    («std::option::Option::map».call h![T, U, E] h![from_option (some v), f])
+    (fun v => (∃∃vin, v = (from_option (some vin)) ⋆ Q vin) ⋆ [λf ↦ fb]) := by
   enter_decl
   steps
-  apply Lampe.STHoare.iteTrue_intro
-  steps [Lampe.STHoare.callLambda_intro (hlam := h_lam), some_spec]
+  apply STHoare.iteTrue_intro
+  steps [STHoare.callLambda_intro (hlam := h_lam), some_spec]
   case _ : _ = _ => assumption
   sl
 
-lemma map_pure_spec {p T U E f fb v f_emb}
-    (h_f: ∀arg, Lampe.STHoare p env ⟦⟧ (fb h![arg]) (fun r => r = f_emb arg)):
-    Lampe.STHoare p env 
-      [λf ↦ fb] 
-      («std::option::Option::map».call h![T, U, E] h![from_option v, f]) 
-      (fun r => r = from_option (v.map f_emb)) := by
+theorem map_pure_spec {p T U E f fb v f_emb}
+    (h_f : ∀arg, STHoare p env ⟦⟧ (fb h![arg]) (fun r => r = f_emb arg))
+  : STHoare p env 
+    [λf ↦ fb] 
+    («std::option::Option::map».call h![T, U, E] h![from_option v, f]) 
+    (fun r => r = from_option (v.map f_emb)) := by
   cases v
   · steps [map_none_spec]
     assumption
   · steps [map_some_spec (h_f _)]
     simp_all
+
+theorem map_or_none_spec {p T U E f default} 
+  : STHoare p env ⟦⟧
+    («std::option::Option::map_or».call h![T, U, E] h![from_option none, default, f])
+    (fun r => r = default) := by
+  enter_decl
+  steps
+  apply STHoare.iteFalse_intro
+  steps
+  assumption
+
+theorem map_or_some_spec {p T U E f v fb P Q default} 
+    (h_lam : STHoare p env P (fb h![v]) Q)
+  : STHoare p env
+    (P ⋆ [λf ↦ fb])
+    («std::option::Option::map_or».call h![T, U, E] h![from_option (some v), default, f])
+    (fun v => Q v ⋆ [λf ↦ fb]) := by
+  enter_decl
+  steps
+  apply STHoare.iteTrue_intro
+  steps [STHoare.callLambda_intro (hlam := h_lam)]
+
+lemma map_or_pure_spec {p T U E f fb v} 
+    {default : U.denote p}
+    {f_emb : T.denote p → U.denote p}
+    (h_f : ∀arg, STHoare p env ⟦⟧ (fb h![arg]) (fun r => r = f_emb arg))
+  : STHoare p env
+    [λf ↦ fb]
+    («std::option::Option::map_or».call h![T, U, E] h![from_option v, default, f])
+    (fun r => r = (v.map f_emb).getD default) := by
+  cases v
+  . steps [map_or_none_spec]
+    assumption
+  . steps [map_or_some_spec (E := E) (h_f _)]
+    simp_all
+    
+
