docs/Tips for Proving.md
@@ -1,0 +1,43 @@
+# Tips for Proving
+
+This document contains some tips for stating and proving theorems about extracted Noir code, and
+aims to be a compendium of useful patterns and knowledge.
+
+## Existing Logic Over Custom Logic
+
+> If you can write a piece of logic using existing Lean functionality, do so.
+
+It is always possible to state program properties in Lean in terms of hand-written logic—such as
+`if`, `match`, and so on—when stating theorems. However, if there is an equivalent to that logic in
+terms of existing types and/or functionality it should always be preferred. This means that
+downstream dependents of that theorem will have as much of the existing set of Lean theorems at 
+their disposal as is possible, rather than having to manually work with the constructs.
+
+An example would be the post-condition for `std::option::Option::map_or`. Using bare, hand-written
+logic, it could be stated as follows:
+
+```lean
+fun r => r = match v with
+| some x => f x
+| none => default
+```
+
+This would mean that a user of the theorem would have to deal with that match explicitly every
+single time it was employed. Alternatively, this can be stated in terms of operations on `Option`.
+
+```lean
+fun r => r = (v.map f).getD default
+```
+
+Constructs such as `Option.map` and `Option.getD` all have significant existing bodies of theorems
+accompanying them, and are hence _much_ more useful in a theorem statement.
+
+## Reason About Lean Types
+
+> Wherever possible, translate the problem statement to be in terms of _Lean_ types and functions
+> instead of Noir ones.
+
+One of the major aims of Lampe is to avoid the need to reason directly about _Noir_ constructs and
+types. Lean constructs have a significant base of theorems and work available with them, that does
+not exist when directly reasoning about Noir's constructs.
+
